Use LowParse for protocolVersion'
***NO_CI***

src/tls/TLSConstants.fst
@@ -519,39 +519,242 @@ let rec compressionMethodsBytes cms =
 
 #set-options "--max_fuel 0 --initial_fuel 0 --max_ifuel 1 --initial_ifuel 1"
 
+module LP = LowParse.SLow
+module L = FStar.List.Tot
+
+let protocolVersion_enum : LP.enum protocolVersion (byte * byte) =
+  let e = [
+    SSL_3p0, (3z, 0z);
+    TLS_1p0, (3z, 1z);
+    TLS_1p1, (3z, 2z);
+    TLS_1p2, (3z, 3z);
+    TLS_1p3, (3z, 4z);
+  ]
+  in
+  assert_norm (L.noRepeats (L.map fst e));
+  assert_norm (L.noRepeats (L.map snd e));
+  e
+
+#set-options "--z3rlimit 32 --max_fuel 16 --initial_fuel 16 --max_ifuel 16 --initial_ifuel 16"
+
+let synth_protocolVersion'
+  (x: LP.maybe_enum_key protocolVersion_enum)
+: Tot protocolVersion'
+= match x with
+  | LP.Known k -> k
+  | LP.Unknown y ->
+    let (a, b) = (y <: (byte * byte)) in
+    UnknownVersion a b
+
+let rec not_mem
+  (#t: eqtype)
+  (x: t)
+  (l: list t)
+: Tot (y: bool { y == true <==> L.mem x l == false } )
+= match l with
+  | [] -> true
+  | a :: q ->
+    let f = not_mem x q in
+    (x <> a && f)
+
+let synth_protocolVersion'_recip
+  (x: protocolVersion')
+: Tot (LP.maybe_enum_key protocolVersion_enum)
+= match x with
+  | UnknownVersion a b ->
+    let (y: (byte * byte)) = (a, b) in
+    assert (normalize_term (not_mem y (L.map snd protocolVersion_enum)) == true);
+    LP.Unknown y
+  | x -> LP.Known x
+
+let synth_protocolVersion'_recip_correct () : Lemma
+  (forall (x: LP.maybe_enum_key protocolVersion_enum) . synth_protocolVersion'_recip (synth_protocolVersion' x) == x)
+= ()
+
+let parse_maybe_protocolVersion_key : LP.parser _ (LP.maybe_enum_key protocolVersion_enum) =
+  LP.parse_maybe_enum_key (LP.parse_u8 `LP.nondep_then` LP.parse_u8) protocolVersion_enum
+
+#set-options "--z3rlimit 64 --max_fuel 32 --initial_fuel 32 --max_ifuel 32 --initial_ifuel 32 --z3refresh"
+
+let synth_protocolVersion'_inj () : Lemma (forall (x1 x2: LP.maybe_enum_key protocolVersion_enum) .
+  synth_protocolVersion' x1 == synth_protocolVersion' x2 ==> x1 == x2)
+= ()
+
+let serialize_maybe_protocolVersion_key : LP.serializer parse_maybe_protocolVersion_key =
+  LP.serialize_maybe_enum_key _ (LP.serialize_nondep_then _ LP.serialize_u8 () _ LP.serialize_u8) protocolVersion_enum
+
+let parse_protocolVersion' : LP.parser _ protocolVersion' =
+  synth_protocolVersion'_inj ();
+  parse_maybe_protocolVersion_key `LP.parse_synth` synth_protocolVersion'
+
+let serialize_protocolVersion' : LP.serializer parse_protocolVersion' =
+  synth_protocolVersion'_inj ();
+  synth_protocolVersion'_recip_correct ();
+  LP.serialize_synth _ synth_protocolVersion'  serialize_maybe_protocolVersion_key synth_protocolVersion'_recip ()
+
+let parse32_maybe_protocolVersion_key : LP.parser32 parse_maybe_protocolVersion_key =
+  LP.parse32_maybe_enum_key_gen
+    (LP.parse32_u8 `LP.parse32_nondep_then` LP.parse32_u8)
+    protocolVersion_enum
+    (normalize_term (LP.maybe_enum_key_of_repr' protocolVersion_enum))
+
+let parse32_protocolVersion' : LP.parser32 parse_protocolVersion' =
+  synth_protocolVersion'_inj () ;
+  LP.parse32_synth
+    _
+    synth_protocolVersion'
+    (fun x -> synth_protocolVersion' x)
+    parse32_maybe_protocolVersion_key
+    ()
+
+let serialize32_maybe_protocolVersion_key : LP.serializer32 serialize_maybe_protocolVersion_key =
+  let s = LP.serialize32_nondep_then #_ #_ #LP.parse_u8 #LP.serialize_u8 LP.serialize32_u8 () #_ #_ #LP.parse_u8 #LP.serialize_u8 LP.serialize32_u8 () in
+  LP.serialize32_maybe_enum_key_gen
+    s
+    protocolVersion_enum
+    (LP.serialize32_enum_key_gen
+      s
+      protocolVersion_enum
+      (normalize_term (LP.enum_repr_of_key' protocolVersion_enum))
+    )
+
+let serialize32_protocolVersion' : LP.serializer32 serialize_protocolVersion' =
+  synth_protocolVersion'_inj ();
+  synth_protocolVersion'_recip_correct ();
+  LP.serialize32_synth
+    _
+    synth_protocolVersion'
+    _
+    serialize32_maybe_protocolVersion_key
+    synth_protocolVersion'_recip
+    (fun x -> synth_protocolVersion'_recip x)
+    ()
+
 (** Serializing function for the protocol version *)
-val versionBytes: protocolVersion' -> Tot (lbytes 2)
-let versionBytes pv =
-  match pv with
-  | SSL_3p0 -> twobytes ( 3z, 0z)
-  | TLS_1p0 -> twobytes ( 3z, 1z)
-  | TLS_1p1 -> twobytes ( 3z, 2z )
-  | TLS_1p2 -> twobytes ( 3z, 3z )
-  | TLS_1p3 -> twobytes ( 3z, 4z )
-  | UnknownVersion a b -> twobytes ( a, b )
+let versionBytes (input: protocolVersion') : Tot (lbytes 2) =
+  serialize32_protocolVersion' input <: LP.bytes32
+
+
+(** TODO: move to LowParse *)
+
+let get_parser_kind
+  (#k: LP.parser_kind)
+  (#t: Type0)
+  (p: LP.parser k t)
+: Tot LP.parser_kind
+= k
+
+let parse32_size
+  (#k: LP.parser_kind)
+  (#t: Type0)
+  (#p: LP.parser k t)
+  (p32: LP.parser32 p)
+  (input: bytes)
+  (data: t)
+  (consumed: UInt32.t)
+: Lemma
+  (requires (p32 input == Some (data, consumed)))
+  (ensures (
+    k.LP.parser_kind_low <= UInt32.v consumed /\ (
+    Some? k.LP.parser_kind_high ==> (
+    let (Some hi) = k.LP.parser_kind_high in
+    UInt32.v consumed <= hi
+  ))))
+= ()
+
+let parse32_total
+  (#k: LP.parser_kind)
+  (#t: Type0)
+  (#p: LP.parser k t)
+  (p32: LP.parser32 p)
+  (input: bytes)
+: Lemma
+  (requires (
+    k.LP.parser_kind_high == Some k.LP.parser_kind_low /\
+    k.LP.parser_kind_total == true /\
+    k.LP.parser_kind_low <= Bytes.length input
+  ))
+  (ensures (
+    Some? (p32 input)
+  ))
+= ()
+
+let bytes_equal_intro
+  (b1 b2: bytes)
+: Lemma
+  (requires (Bytes.reveal b1 == Bytes.reveal b2))
+  (ensures (Bytes.equal b1 b2))
+= ()
+
+let parser32_then_serializer32'
+  (#k: LP.parser_kind)
+  (#t: Type0)
+  (#p: LP.parser k t)
+  (#s: LP.serializer p)
+  (p32: LP.parser32 p)
+  (s32: LP.serializer32 s)
+  (input: bytes)
+  (v: t)
+  (consumed: UInt32.t)
+: Lemma
+  (requires (p32 input == Some (v, consumed)))
+  (ensures (
+    Bytes.length (s32 v) == UInt32.v consumed /\
+    Bytes.reveal (s32 v) == Seq.slice (Bytes.reveal input) 0 (UInt32.v consumed)
+  ))
+= admit ()
+
+let le_antisym (x1 x2: int) : Lemma (requires (x1 <= x2 /\ x2 <= x1)) (ensures (x1 == x2)) = ()
+
+(** END TODO: move *)
 
 (** Parsing function for the protocol version *)
+(* NOTE: this interface (as well as versionBytes) is dubious, since:
+   - it makes explicit the size of bytes to parse
+   - nothing tells that all input bytes were actually consumed
+   In particular, this interface means that the caller is responsible for correctly splitting the input buffer *before* calling the parser.
+*)
 val parseVersion: pinverse_t versionBytes
 let parseVersion v =
-  match cbyte2 v with
-  | ( 3z, 0z ) -> Correct SSL_3p0
-  | ( 3z, 1z ) -> Correct TLS_1p0
-  | ( 3z, 2z ) -> Correct TLS_1p1
-  | ( 3z, 3z ) -> Correct TLS_1p2
-  | ( 3z, 4z ) -> Correct TLS_1p3
-  | ( a,  b  ) -> Correct (UnknownVersion a b)
+  parse32_total parse32_protocolVersion' v;
+  let (Some (value, _)) = parse32_protocolVersion' v in
+  Correct value
 
+(* The following surprisingly succeeds. *)
 val inverse_version: x:_ -> Lemma
   (requires True)
   (ensures lemma_inverse_g_f versionBytes parseVersion x)
   [SMTPat (parseVersion (versionBytes x))]
 let inverse_version x = ()
 
-val pinverse_version: x:_ -> Lemma
+val pinverse_version: x: lbytes 2 -> Lemma
   (requires True)
   (ensures (lemma_pinverse_f_g Bytes.equal versionBytes parseVersion x))
   [SMTPat (versionBytes (Correct?._0 (parseVersion x)))]
-let pinverse_version x = ()
+
+(* The following fails, as expected. *)
+// let pinverse_version x = ()
+(* We have to call an explicit lemma, albeit generic *)
+
+let pinverse_version x =
+  parse32_total parse32_protocolVersion' x;
+  let (Correct c) = parseVersion x in
+  let (Some (c', consumed)) = parse32_protocolVersion' x in
+  assert (c == c');
+  let f () : Lemma (2 <= UInt32.v consumed /\ UInt32.v consumed <= 2) =
+    let k = get_parser_kind parse_protocolVersion' in
+    assert (k.LP.parser_kind_low == 2);
+    assert (k.LP.parser_kind_high == Some 2);
+    parse32_size #k #protocolVersion' #parse_protocolVersion' parse32_protocolVersion' x c consumed;
+    ()
+  in
+  f ();
+  le_antisym (UInt32.v consumed) 2;
+  assert (UInt32.v consumed == 2);
+  parser32_then_serializer32' parse32_protocolVersion' serialize32_protocolVersion' x c' consumed;
+  ()
+
+#set-options "--max_fuel 0 --initial_fuel 0 --max_ifuel 1 --initial_ifuel 1"
 
 // DRAFT#21
 // to be used *only* in ServerHello.version.
